spc/RobustIndexedInvariants.v
@@ -2,7 +2,486 @@ From stdpp Require Import coPset gmap namespaces.
 From sflib Require Import sflib.
 From iris Require Import bi.big_op.
 From iris Require base_logic.lib.invariants.
-Require Import PCM IProp IPM.
+
+Require Import Coqlib PCM IProp IPM.
+
+Require Import Coq.Logic.ClassicalEpsilon.
+Require Import Coq.Logic.IndefiniteDescription.
+
+(* Require ClassicalFacts. *)
+(* Require FunctionalExtensionality. *)
+(* Require ChoiceFacts. *)
+(* Require Coq.Logic.Epsilon. *)
+(* Require Classical_Prop. *)
+(* Require Logic.Classical_Pred_Type. *)
+(* Require Import Coq.Logic.ProofIrrelevance. *)
+(* Require Import Coq.Logic.ClassicalEpsilon. *)
+
+
+
+
+Lemma dependent_functional_choice (A : Type) (B : A -> Type) :
+  forall R : forall x : A, B x -> Prop,
+    (forall x : A, exists y : B x, R x y) ->
+    (exists f : (forall x : A, B x), forall x : A, R x (f x)).
+Proof.
+  eapply ChoiceFacts.non_dep_dep_functional_choice.
+  clear. exact functional_choice.
+Qed.  
+
+
+
+Section POINTWISE.
+
+  Lemma unfold_pointwise_add X (M: URA.t) (f0 f1: (X ==> M)%ra)
+    :
+    f0 ⋅ f1 = (fun x => f0 x ⋅ f1 x).
+  Proof.
+    ur. ur. auto.
+  Qed.
+
+  Lemma updatable_set_impl (M: URA.t)
+        (P0 P1: M -> Prop)
+        (IMPL: forall r, URA.wf r -> P0 r -> P1 r)
+        (m: M)
+        (UPD: URA.updatable_set m P0)
+    :
+    URA.updatable_set m P1.
+  Proof.
+    ii. eapply UPD in WF; eauto. des.
+    esplits; eauto. eapply IMPL; auto.
+    eapply URA.wf_mon. eauto.
+  Qed.
+
+  Lemma pointwise_extends A (M: URA.t)
+        (f0 f1: (A ==> M)%ra)
+        (UPD: forall a, URA.extends (f0 a) (f1 a))
+    :
+    URA.extends f0 f1.
+  Proof.
+    hexploit (choice (fun a ctx => f1 a = ((f0 a) ⋅ ctx))).
+    { i. specialize (UPD x). r in UPD. des. eauto. }
+    i. des. exists f.
+    rewrite (@unfold_pointwise_add A M). extensionality a. auto.
+  Qed.
+
+  Lemma pointwise_updatable A (M: URA.t)
+        (f0 f1: (A ==> M)%ra)
+        (UPD: forall a, URA.updatable (f0 a) (f1 a))
+    :
+    URA.updatable f0 f1.
+  Proof.
+    ii. ur. i. ur in H. specialize (H k).
+    eapply (UPD k); eauto.
+  Qed.
+
+  Lemma pointwise_updatable_set A (M: URA.t)
+        (f: (A ==> M)%ra)
+        (P: A -> M -> Prop)
+        (UPD: forall a, URA.updatable_set (f a) (P a))
+    :
+    URA.updatable_set f (fun f' => forall a, P a (f' a)).
+  Proof.
+    ii. hexploit (choice (fun a m => P a m /\ URA.wf (m ⋅ ctx a))).
+    { i. eapply (UPD x). ur in WF. auto. }
+    i. des. exists f0. splits; auto.
+    { i. specialize (H a). des. auto. }
+    { ur. i. specialize (H k). des. auto. }
+  Qed.
+
+  Definition maps_to_res {A} {M: URA.t}
+             a m: (A ==> M)%ra :=
+    fun a' => if excluded_middle_informative (a' = a)
+              then m
+              else URA.unit.
+
+  Lemma maps_to_res_add A (M: URA.t)
+        (a: A) (m0 m1: M)
+    :
+    maps_to_res a m0 ⋅ maps_to_res a m1
+    =
+      maps_to_res a (m0 ⋅ m1).
+  Proof.
+    extensionality a'. unfold maps_to_res. ur. des_ifs.
+    { ur. auto. }
+    { r_solve. }
+  Qed.
+
+  Lemma maps_to_updatable A (M: URA.t)
+        (a: A) (m0 m1: M)
+        (UPD: URA.updatable m0 m1)
+    :
+    URA.updatable (maps_to_res a m0) (maps_to_res a m1).
+  Proof.
+    eapply pointwise_updatable. i.
+    unfold maps_to_res. des_ifs.
+  Qed.
+
+  Lemma maps_to_updatable_set A (M: URA.t)
+        (a: A) (m: M) (P: M -> Prop)
+        (UPD: URA.updatable_set m P)
+    :
+    URA.updatable_set
+      (maps_to_res a m)
+      (fun f => exists (m1: M), f = maps_to_res a m1 /\ P m1).
+  Proof.
+    eapply updatable_set_impl; cycle 1.
+    { eapply pointwise_updatable_set.
+      instantiate (1:= fun a' m' => (a' = a -> P m') /\ (a' <> a -> m' = URA.unit)).
+      ii. unfold maps_to_res in WF. des_ifs.
+      { exploit UPD; eauto. i. des. esplits; eauto. ss. }
+      { exists URA.unit. splits; ss. }
+    }
+    { i. ss. exists (r a). splits; auto.
+      { extensionality a'. unfold maps_to_res. des_ifs.
+        specialize (H0 a'). des. auto.
+      }
+      { specialize (H0 a). des. auto. }
+    }
+  Qed.
+
+  Definition map_update {A} {M: URA.t}
+             (f: (A ==> M)%ra) a m :=
+    fun a' => if excluded_middle_informative (a' = a)
+              then m
+              else f a'.
+
+End POINTWISE.
+
+Global Opaque URA.unit.
+
+Section UNIT.
+
+  Program Instance Unit : URA.t := {| URA.unit := tt; URA._add := fun _ _ => tt; URA._wf := fun _ => True; URA.core := fun _ => tt; |}.
+  Next Obligation. destruct a. ss. Qed.
+  Next Obligation. destruct a. ss. Qed.
+  Next Obligation. unseal "ra". i. destruct a. ss. Qed.
+  Next Obligation. unseal "ra". ss. Qed.
+  Next Obligation. unseal "ra". i. ss. Qed.
+  Next Obligation. unseal "ra". i. destruct a. ss. Qed.
+  Next Obligation. ss. Qed.
+  Next Obligation. unseal "ra". i. exists tt. ss. Qed.
+
+  Lemma Unit_wf : forall x, @URA.wf Unit x.
+  Proof. unfold URA.wf. unseal "ra". ss. Qed.
+
+End UNIT.
+Global Opaque Unit.
+
+
+Section URA_PROD.
+
+  Lemma unfold_prod_add (M0 M1 : URA.t) : @URA.add (URA.prod M0 M1) = fun '(a0, a1) '(b0, b1) => (a0 ⋅ b0, a1 ⋅ b1).
+  Proof. rewrite URA.unfold_add. extensionalities r0 r1. destruct r0, r1. ss. Qed.
+
+  Lemma unfold_prod_wf (M0 M1 : URA.t) : @URA.wf (URA.prod M0 M1) = fun r => URA.wf (fst r) /\ URA.wf (snd r).
+  Proof. rewrite URA.unfold_wf. extensionalities r. destruct r. ss. Qed.
+
+End URA_PROD.
+
+Section PWDEP.
+
+  Lemma pointwise_dep_updatable
+        A (Ms : A -> URA.t)
+        (f0 f1 : @URA.pointwise_dep A Ms)
+        (UPD : forall a, URA.updatable (f0 a) (f1 a))
+    :
+    URA.updatable f0 f1.
+  Proof.
+    ii. ur. i. ur in H. specialize (H k).
+    eapply (UPD k); eauto.
+  Qed.
+
+  Lemma pointwise_dep_updatable_set
+        A (Ms : A -> URA.t)
+        (f : @URA.pointwise_dep A Ms)
+        (P : forall (a : A), (Ms a) -> Prop)
+        (UPD: forall a, URA.updatable_set (f a) (P a))
+    :
+    URA.updatable_set f (fun f' => forall a, P a (f' a)).
+  Proof.
+    ii.
+    set (R := fun (a : A) => (fun (m : Ms a) => P a m /\ URA.wf (m ⋅ ctx a))).
+    hexploit (dependent_functional_choice _ _ R).
+    { subst R. ss. i. eapply (UPD x). ur in WF. auto. }
+    subst R. ss. i. des. exists f0. splits; auto.
+    { i. specialize (H a). des. auto. }
+    { ur. i. specialize (H k). des. auto. }
+  Qed.
+
+  Program Definition maps_to_res_dep {A : Type} {Ms : A -> URA.t} (a : A) (m : Ms a)
+    : @URA.pointwise_dep A Ms.
+  Proof.
+    ii. destruct (excluded_middle_informative (k = a)).
+    - subst k. exact m.
+    - exact ε.
+  Defined.
+
+  Lemma maps_to_res_dep_eq
+        A (Ms : A -> URA.t)
+        (a : A)
+        (m : Ms a)
+    :
+    (@maps_to_res_dep A Ms a m) a = m.
+  Proof.
+    unfold maps_to_res_dep. des_ifs. unfold eq_rect_r.
+    rewrite <- Eqdep.EqdepTheory.eq_rect_eq. auto.
+  Qed.
+
+  Lemma maps_to_res_dep_neq
+        A (Ms : A -> URA.t)
+        (a b : A)
+        (m : Ms a)
+    :
+    a <> b -> (@maps_to_res_dep A Ms a m) b = ε.
+  Proof.
+    i. unfold maps_to_res_dep. des_ifs.
+  Qed.
+
+  Lemma maps_to_res_dep_add
+        A (Ms : A -> URA.t)
+        (a : A)
+        (m0 m1 : Ms a)
+    :
+    @maps_to_res_dep _ Ms a m0 ⋅ @maps_to_res_dep _ Ms a m1 = @maps_to_res_dep _ Ms a (m0 ⋅ m1).
+  Proof.
+    extensionalities a'. unfold URA.add at 1. unseal "ra". ss.
+    destruct (excluded_middle_informative (a' = a)).
+    - subst a'. rewrite ! @maps_to_res_dep_eq. auto.
+    - rewrite ! @maps_to_res_dep_neq; auto. apply URA.unit_id.
+  Qed.
+
+  Lemma maps_to_res_dep_updatable
+        A (Ms : A -> URA.t)
+        (a : A)
+        (m0 m1 : Ms a)
+        (UPD: URA.updatable m0 m1)
+    :
+    URA.updatable (@maps_to_res_dep A Ms a m0) (@maps_to_res_dep A Ms a m1).
+  Proof.
+    eapply pointwise_dep_updatable. i. unfold maps_to_res_dep. des_ifs.
+  Qed.
+
+  Lemma maps_to_res_dep_updatable_set
+        A (Ms : A -> URA.t)
+        (a : A)
+        (m : Ms a)
+        (P : forall (a' : A), Ms a' -> Prop)
+        (UPD: URA.updatable_set m (P a))
+    :
+    URA.updatable_set
+      (@maps_to_res_dep A Ms a m)
+      (fun f => exists (m1 : Ms a), f = @maps_to_res_dep A Ms a m1 /\ (P a m1)).
+  Proof.
+    eapply updatable_set_impl; cycle 1.
+    { eapply pointwise_dep_updatable_set.
+      instantiate (1:= fun a' m' => (a' = a -> P a' m') /\ (a' <> a -> m' = URA.unit)).
+      ii. unfold maps_to_res_dep in WF. des_ifs.
+      { exploit UPD; eauto. i. des. esplits; eauto. ss. }
+      { exists URA.unit. splits; ss. }
+    }
+    { i. ss. exists (r a). splits; auto.
+      { extensionalities a'. unfold maps_to_res_dep. des_ifs.
+        specialize (H0 a'). des. auto.
+      }
+      { specialize (H0 a). des. auto. }
+    }
+  Qed.
+
+  Program Definition maps_to_res_dep_update {A} {Ms: A -> URA.t}
+          (f: @URA.pointwise_dep A Ms) a (m : Ms a) : @URA.pointwise_dep A Ms.
+  Proof.
+    ii. destruct (excluded_middle_informative (k = a)).
+    - subst k. exact m.
+    - exact (f k).
+  Qed.
+
+End PWDEP.
+
+
+
+Tactic Notation "unfold_prod" :=
+  try rewrite ! unfold_prod_add;
+  rewrite unfold_prod_wf;
+  simpl.
+
+Tactic Notation "unfold_prod" hyp(H) :=
+  try rewrite ! unfold_prod_add in H;
+  rewrite unfold_prod_wf in H;
+  simpl in H;
+  let H1 := fresh H in
+  destruct H as [H H1].
+
+From iris.bi Require Import derived_connectives updates.
+From iris.prelude Require Import options.
+
+Section PWAUX.
+
+  Context {K: Type} `{M: URA.t}.
+  Let RA := URA.pointwise K M.
+
+  Lemma pw_extends (f0 f1: K -> M) (EXT: @URA.extends RA f0 f1): <<EXT: forall k, URA.extends (f0 k) (f1 k)>>.
+  Proof. ii. r in EXT. des. subst. ur. ss. eexists; eauto. Qed.
+
+  Lemma pw_wf: forall (f: K -> M) (WF: URA.wf (f: @URA.car RA)), <<WF: forall k, URA.wf (f k)>>.
+  Proof. ii; ss. rewrite URA.unfold_wf in WF. ss. Qed.
+
+  Lemma pw_add_disj_wf
+        (f g: K -> M)
+        (WF0: URA.wf (f: @URA.car RA))
+        (WF1: URA.wf (g: @URA.car RA))
+        (DISJ: forall k, <<DISJ: f k = ε \/ g k = ε>>)
+    :
+      <<WF: URA.wf ((f: RA) ⋅ g)>>
+  .
+  Proof.
+    ii; ss. ur. i. ur in WF0. ur in WF1. specialize (DISJ k). des; rewrite DISJ.
+    - rewrite URA.unit_idl; eauto.
+    - rewrite URA.unit_id; eauto.
+  Qed.
+
+  Lemma pw_insert_wf: forall `{EqDecision K} (f: K -> M) k v (WF: URA.wf (f: @URA.car RA)) (WFV: URA.wf v),
+      <<WF: URA.wf (<[k:=v]> f: @URA.car RA)>>.
+  Proof.
+    i. unfold insert, functions.fn_insert. ur. ii. des_ifs. ur in WF. eapply WF.
+  Qed.
+
+  Lemma pw_lookup_wf: forall (f: @URA.car RA) k (WF: URA.wf f), URA.wf (f k).
+  Proof. ii; ss. rewrite URA.unfold_wf in WF. ss. Qed.
+
+End PWAUX.
+
+Section PWDAUX.
+
+  Context {K: Type} `{M: K -> URA.t}.
+  Let RA := @URA.pointwise_dep K M.
+
+  Lemma pwd_extends (f0 f1: forall (k : K), M k) (EXT: @URA.extends RA f0 f1): <<EXT: forall k, URA.extends (f0 k) (f1 k)>>.
+  Proof. ii. r in EXT. des. subst. ur. ss. eexists; eauto. Qed.
+
+  Lemma pwd_wf: forall (f: forall (k : K), M k) (WF: URA.wf (f: @URA.car RA)), <<WF: forall k, URA.wf (f k)>>.
+  Proof. ii; ss. rewrite URA.unfold_wf in WF. ss. Qed.
+
+  Lemma pwd_add_disj_wf
+        (f g: forall (k : K), M k)
+        (WF0: URA.wf (f: @URA.car RA))
+        (WF1: URA.wf (g: @URA.car RA))
+        (DISJ: forall k, <<DISJ: f k = ε \/ g k = ε>>)
+    :
+      <<WF: URA.wf ((f: RA) ⋅ g)>>
+  .
+  Proof.
+    ii; ss. ur. i. ur in WF0. ur in WF1. specialize (DISJ k). des; rewrite DISJ.
+    - rewrite URA.unit_idl; eauto.
+    - rewrite URA.unit_id; eauto.
+  Qed.
+
+  Lemma pwd_lookup_wf: forall (f: @URA.car RA) k (WF: URA.wf f), URA.wf (f k).
+  Proof. ii; ss. rewrite URA.unfold_wf in WF. ss. Qed.
+
+End PWDAUX.
+
+Module Gset.
+  Import gmap.
+
+  Definition add (x y : option (gset positive)) : option (gset positive) :=
+    match x, y with
+    | Some x, Some y => if decide (x ## y) then Some (x ∪ y) else None
+    | _, _ => None
+    end.
+
+  Program Instance t : URA.t :=
+    {|
+      URA.car := option (gset positive);
+      URA.unit := Some ∅;
+      URA._wf := fun x => match x with Some _ => True | None => False end;
+      URA._add := add;
+      URA.core := fun x => Some ∅;
+    |}.
+  Next Obligation.
+    unfold add. intros [] []; des_ifs. f_equal. set_solver.
+  Qed.
+  Next Obligation.
+    unfold add. intros [] [] []; des_ifs.
+    { f_equal. set_solver. }
+    all: set_solver.
+  Qed.
+  Next Obligation.
+    unseal "ra". unfold add. intros []; des_ifs.
+    { f_equal. set_solver. }
+    set_solver.
+  Qed.
+  Next Obligation.
+    unseal "ra". ss.
+  Qed.
+  Next Obligation.
+    unseal "ra". ss. intros [] []; ss.
+  Qed.
+  Next Obligation.
+    unseal "ra". ss. intros []; des_ifs.
+    { f_equal. set_solver. }
+    set_solver.
+  Qed.
+  Next Obligation.
+    intros []; ss.
+  Qed.
+  Next Obligation.
+    unseal "ra". i. exists (Some ∅). ss. des_ifs.
+    { f_equal. set_solver. }
+    set_solver.
+  Qed.
+
+End Gset.
+
+
+Module CoPset.
+
+  Definition add (x y : option coPset) : option coPset :=
+    match x, y with
+    | Some x, Some y => if decide (x ## y) then Some (x ∪ y) else None
+    | _, _ => None
+    end.
+
+  Program Instance t : URA.t :=
+    {|
+      URA.car := option coPset;
+      URA.unit := Some ∅;
+      URA._wf := fun x => match x with Some _ => True | None => False end;
+      URA._add := add;
+      URA.core := fun x => Some ∅;
+    |}.
+  Next Obligation.
+    intros [] []; ss. des_ifs. f_equal. set_solver.
+  Qed.
+  Next Obligation.
+    unfold add. intros [] [] []; des_ifs.
+    { f_equal. set_solver. }
+    all: set_solver.
+  Qed.
+  Next Obligation.
+    unseal "ra". unfold add. intros []; des_ifs.
+    - f_equal. set_solver.
+    - set_solver.
+  Qed.
+  Next Obligation.
+    unseal "ra". ss.
+  Qed.
+  Next Obligation.
+    unseal "ra". intros [] []; ss.
+  Qed.
+  Next Obligation.
+    unseal "ra". unfold add. intros []; des_ifs.
+    - f_equal. set_solver.
+    - set_solver.
+  Qed.
+  Next Obligation.
+    intros []; ss.
+  Qed.
+  Next Obligation.
+    unseal "ra". i. exists (Some ∅). ss. f_equal. set_solver.
+  Qed.
+
+End CoPset.
 
 Local Notation index := nat.
 
@@ -110,7 +589,7 @@ Section PCM_OWN.
     remember (@maps_to_res_dep index (InvSetRA Vars) n (Auth.white (@maps_to_res positive (URA.agree (Vars n)) i (Some (Some p))))) as r.
     unfold Persistent. iIntros "H".
     iPoseProof (@OwnM_persistently _ _ H _ with "H") as "#HP". iModIntro.
-    replace r with (URA.core r) at 2. auto.
+    replace r with (URA.core r) at 2; auto.
     subst. unfold maps_to_res_dep, maps_to_res. ss. extensionalities k. des_ifs.
   Qed.
 
@@ -229,7 +708,7 @@ Section WORLD_SATISFACTION.
     : wsat ∗ prop n p ⊢ |==> (∃ i, ⌜φ i⌝ ∧ OwnI n i p) ∗ wsat.
   Proof.
     iIntros "[W P]".
-    iMod (wsat_OwnI_alloc_gen with "W") as "[I W]". eauto.
+    iMod (wsat_OwnI_alloc_gen with "W") as "[I W]"; eauto.
     iFrame. iModIntro. iApply "W". iFrame.
   Qed.
 
@@ -242,7 +721,7 @@ Section WORLD_SATISFACTION.
     iPoseProof (OwnM_valid with "AUTH") as "%WF".
     assert (Hip : I !! i = Some p).
     { unfold inv_auth_black, OwnI_white in WF. setoid_rewrite maps_to_res_dep_add in WF.
-      unfold maps_to_res_dep, maps_to_res in WF. apply (pwd_lookup_wf n) in WF. ss. des_ifs.
+      unfold maps_to_res_dep, maps_to_res in WF. apply (pwd_lookup_wf _ n) in WF. ss. des_ifs.
       unfold eq_rect_r in WF. rewrite <- Eqdep.EqdepTheory.eq_rect_eq in WF.
       apply Auth.auth_included in WF. rename WF into EXTENDS.
       apply pw_extends in EXTENDS. specialize (EXTENDS i).
@@ -272,7 +751,7 @@ Section WORLD_SATISFACTION.
     iPoseProof (OwnM_valid with "AUTH") as "%WF".
     assert (Hip : I !! i = Some p).
     { unfold inv_auth_black, OwnI_white in WF. setoid_rewrite maps_to_res_dep_add in WF.
-      unfold maps_to_res_dep, maps_to_res in WF. apply (pwd_lookup_wf n) in WF. ss. des_ifs.
+      unfold maps_to_res_dep, maps_to_res in WF. apply (pwd_lookup_wf _ n) in WF. ss. des_ifs.
       unfold eq_rect_r in WF. rewrite <- Eqdep.EqdepTheory.eq_rect_eq in WF.
       apply Auth.auth_included in WF. rename WF into EXTENDS.
       apply pw_extends in EXTENDS. specialize (EXTENDS i).
@@ -403,10 +882,10 @@ Section WSATS.
       }
       unfold wsat_auth. rewrite H3. iDestruct "AUTH" as "[AUTH NEW]".
       unfold OwnDs_auth. rewrite H4. iDestruct "DA" as "[DA NEWD]".
-      iPoseProof (wsat_init with "[NEWD NEW]") as "NEW". iFrame.
+      iPoseProof (wsat_init with "[NEWD NEW]") as "NEW"; iFrame.
       subst x. iFrame.
       replace (S n - n) with 1 by lia. ss. iFrame.
-    - iIntros "[DA AUTH]". iPoseProof (IHNIN with "[DA AUTH]") as "[DA [AUTH SAT]]". iFrame.
+    - iIntros "[DA AUTH]". iPoseProof (IHNIN with "[DA AUTH]") as "[DA [AUTH SAT]]"; iFrame.
       clear IHNIN. remember (S m) as y.
       assert ((wsat_auth_black m) =
                 ((wsat_auth_black y)
@@ -446,7 +925,7 @@ Section WSATS.
       }
       unfold wsat_auth. rewrite H3. iDestruct "AUTH" as "[AUTH NEW]".
       unfold OwnDs_auth. rewrite H4. iDestruct "DA" as "[DA NEWD]".
-      iPoseProof (wsat_init with "[NEWD NEW]") as "NEW". iFrame.
+      iPoseProof (wsat_init with "[NEWD NEW]") as "NEW"; iFrame.
       subst y. iFrame.
       replace (S m - x) with ((m - x) + 1) by lia. rewrite seq_app.
       iApply big_sepL_app. iFrame.
@@ -457,7 +936,7 @@ Section WSATS.
     : wsats x ∗ ([∗ list] m ∈ (seq x (n - x)), wsat m) ⊢ wsats n.
   Proof.
     iIntros "[SALL WSAT]". unfold wsats.
-    replace n with (x + (n - x)) by lia. rewrite seq_app. iFrame.
+    replace n with (x + (n - x)) by lia. rewrite seq_app; iFrame.
     replace (x + (n - x) - x) with (n - x) by lia. iFrame.
   Qed.
 
@@ -475,8 +954,8 @@ Section WSATS.
     OwnDs_auth x1 ∗ wsat_auth x1 ∗ wsats x1 ⊢ (OwnDs_auth x2 ∗ wsat_auth x2 ∗ wsats x2).
   Proof.
     iIntros (LT) "(DA & AUTH & SAT)".
-    iPoseProof ((wsat_auth_nin _ _ LT) with "[DA AUTH]") as "(DA & AUTH & NEW)". iFrame.
-    iPoseProof ((wsats_nin _ _ LT) with "[SAT NEW]") as "SAT". iFrame. iFrame.
+    iPoseProof ((wsat_auth_nin _ _ LT) with "[DA AUTH]") as "(DA & AUTH & NEW)"; iFrame.
+    iPoseProof ((wsats_nin _ _ LT) with "[SAT NEW]") as "SAT"; iFrame.
   Qed.
 
 
@@ -490,9 +969,10 @@ Section WSATS.
   Proof.
     iIntros "SALL".
     iPoseProof (big_sepL_lookup_acc with "SALL") as "[WSAT K]".
-    apply lookup_seq_lt; eauto.
-    iPoseProof (wsat_OwnI_alloc_gen with "WSAT") as ">[RES WSAT]". apply INF. iFrame.
-    iModIntro. iIntros "P". iFrame. iPoseProof ("WSAT" with "P") as "WSAT".
+    { apply lookup_seq_lt; eauto. }
+    iPoseProof (wsat_OwnI_alloc_gen with "WSAT") as ">[RES WSAT]".
+    { apply INF. }
+    iFrame. iModIntro. iIntros "P". iFrame. iPoseProof ("WSAT" with "P") as "WSAT".
     iPoseProof ("K" with "WSAT") as "SALL". iFrame.
   Qed.
 
@@ -519,8 +999,10 @@ Section WSATS.
                          ∗ OwnDs_auth (S n) ∗ wsat_auth (S n) ∗ (prop n p -∗ wsats (S n))).
   Proof.
     iIntros "(DA & AUTH & WSAT)".
-    iPoseProof ((wsats_allocs x (S n)) with "[DA AUTH WSAT]") as "[DA [AUTH WSAT]]". lia. iFrame.
-    iMod ((wsats_OwnI_alloc_lt_gen (S n) n) with "WSAT") as "[RES WSAT]". auto. eauto.
+    iPoseProof ((wsats_allocs x (S n)) with "[DA AUTH WSAT]") as "[DA [AUTH WSAT]]".
+    { lia. }
+    { iFrame. }
+    iMod ((wsats_OwnI_alloc_lt_gen (S n) n) with "WSAT") as "[RES WSAT]"; eauto.
     iModIntro. iFrame.
   Qed.
 
@@ -536,7 +1018,8 @@ Section WSATS.
   Proof.
     iIntros "(D & A & W & P)". iMod (wsats_OwnI_alloc_ge_gen with "[D A W]") as "(I & D & A & W)".
     1,2: eauto.
-    iFrame. iModIntro. iFrame. iApply "W". iFrame.
+    { iFrame. }
+    iModIntro. iFrame. iApply "W". iFrame.
   Qed.
 
   Lemma wsat_auth_OwnI_le x n i p :
@@ -548,7 +1031,7 @@ Section WSATS.
     iPoseProof (OwnM_valid with "AUTH") as "%WF".
     unfold wsat_auth_black, OwnI_white, maps_to_res_dep in WF.
     unfold URA.add in WF. unseal "ra". ss.
-    apply (pwd_lookup_wf n) in WF. ss. des_ifs.
+    apply (pwd_lookup_wf _ n) in WF. ss. des_ifs.
     exfalso. unfold eq_rect_r in WF. rewrite <- Eqdep.EqdepTheory.eq_rect_eq in WF.
     unfold maps_to_res in WF. apply Auth.auth_included in WF. rename WF into EXTENDS.
     apply pw_extends in EXTENDS. specialize (EXTENDS i). des_ifs.
@@ -562,8 +1045,8 @@ Section WSATS.
     iIntros (LT) "(I & SAT & EN)".
     unfold OwnI, wsats.
     iPoseProof (big_sepL_lookup_acc with "SAT") as "[WSAT K]".
-    apply lookup_seq_lt; eauto.
-    ss. iMod (wsat_OwnI_open with "[I WSAT EN]") as "[P [WSAT DN]]". iFrame.
+    { apply lookup_seq_lt; eauto. }
+    ss. iMod (wsat_OwnI_open with "[I WSAT EN]") as "[P [WSAT DN]]". { iFrame. }
     iPoseProof ("K" with "WSAT") as "SAT".
     iModIntro. iFrame.
   Qed.
@@ -573,8 +1056,8 @@ Section WSATS.
   Proof.
     iIntros (LT) "(I & SAT & P & DIS)".
     iPoseProof (big_sepL_lookup_acc with "SAT") as "[WSAT K]".
-    apply lookup_seq_lt; eauto.
-    iMod (wsat_OwnI_close with "[I WSAT P DIS]") as "[WSAT EN]". iFrame.
+    { apply lookup_seq_lt; eauto. }
+    iMod (wsat_OwnI_close with "[I WSAT P DIS]") as "[WSAT EN]". { iFrame. }
     iPoseProof ("K" with "WSAT") as "SAT".
     iModIntro. iFrame.
   Qed.
@@ -664,7 +1147,7 @@ Section OWNES.
   Lemma OwnEs_acc_new Es n (NIN : Es !! n = None) :
     OwnEs Es ⊢ |==> OwnE n ⊤ ∗ OwnEs (<[n := ∅]>Es).
   Proof.
-    iIntros "ENS". iMod (OwnEs_alloc with "ENS") as "ENS". eauto.
+    iIntros "ENS". iMod (OwnEs_alloc with "ENS") as "ENS"; eauto.
     iModIntro.
     assert (<[n:=∅]> Es = <[n:=∅]> (<[n:=⊤]> Es)).
     { rewrite insert_insert. auto. }
@@ -696,7 +1179,8 @@ Section OWNES.
   Lemma OwnEs_free Es n :
     Es !! n = None -> OwnEs (<[n:=⊤]>Es) ⊢ |==> OwnEs Es.
   Proof.
-    iIntros (NIN) "ENS". iPoseProof (OwnEs_acc_in with "ENS") as "[EN ENS]". apply lookup_insert.
+    iIntros (NIN) "ENS". iPoseProof (OwnEs_acc_in with "ENS") as "[EN ENS]".
+    { apply lookup_insert. }
     rewrite insert_insert. unfold OwnEs. iDestruct "ENS" as "[AUTH SAT]".
     iSplitL "EN AUTH".
     - unfold OwnE_auth, OwnE. iCombine "EN AUTH" as "AUTH".
@@ -724,7 +1208,7 @@ Section OWNES.
     { apply lookup_insert. }
     iPoseProof ("IMPL" with "E") as "E".
     iEval (rewrite insert_insert) in "K".
-    iPoseProof (OwnEs_union with "[E K]") as "E". iFrame.
+    iPoseProof (OwnEs_union with "[E K]") as "E". { iFrame. }
     replace (∅ ∪ E2) with E2 by set_solver.
     iFrame.
   Qed.
@@ -733,7 +1217,7 @@ Section OWNES.
     (E1 ⊆ E2) -> OwnEs (<[n:=E2]>Es) ⊢ OwnEs (<[n:=E1]>Es).
   Proof.
     iIntros (SUB) "ES". iApply (OwnEs_update_one with "ES").
-    iIntros "E". iPoseProof (OwnE_subset with "E") as "[E1 _]". eauto. iFrame.
+    iIntros "E". iPoseProof (OwnE_subset with "E") as "[E1 _]"; eauto.
   Qed.
 
   Lemma OwnEs_disjoint Es n E1 E2 :
@@ -752,7 +1236,7 @@ Section OWNES.
     pattern Es. revert Es. apply map_ind.
     { iIntros (TOP) "ES". ss. }
     iIntros (? ? ? NONE IND TOP) "ES".
-    iMod (OwnEs_free with "[ES]") as "ES". eauto.
+    iMod (OwnEs_free with "[ES]") as "ES"; eauto.
     { eapply map_Forall_lookup_1 in TOP. 2: apply lookup_insert. iApply OwnEs_subset; eauto. }
     iApply IND. 2: iFrame.
     eapply map_Forall_insert_1_2; eauto.
@@ -807,8 +1291,8 @@ Section FANCY_UPDATE.
   Proof.
     iIntros (LT) "FUPD (A & SAT & EN)".
     iPoseProof ((wsats_in _ _ LT) with "SAT") as "[SAT K]".
-    iMod ("FUPD" with "[A SAT EN]") as "(A & SAT & EN & P)". iFrame.
-    iModIntro. iFrame. iApply wsats_nin. apply LT. iFrame.
+    iMod ("FUPD" with "[A SAT EN]") as "(A & SAT & EN & P)". { iFrame. }
+    iModIntro. iFrame. iApply wsats_nin; [apply LT | iFrame].
   Qed.
 
   Lemma wsats_inv_gen x A Es n N p :
@@ -825,15 +1309,15 @@ Section FANCY_UPDATE.
     n < x -> (inv n N p -∗ prop n p) ⊢ FUpd x A Es Es (inv n N p).
   Proof.
     iIntros (LT) "P (A & WSAT & EN)".
-    iMod (wsats_inv_gen with "[A WSAT EN]") as "(A & W & EN & #INV)". eauto.
-    iSplitL "A". iApply "A". iFrame.
+    iMod (wsats_inv_gen with "[A WSAT EN]") as "(A & W & EN & #INV)". { eauto. }
+    { iSplitL "A".  { iApply "A". }  iFrame. }
     iPoseProof ("P" with "INV") as "P". iPoseProof ("W" with "P") as "W". iModIntro. iFrame. auto.
   Qed.
 
   Lemma FUpd_alloc x A Es n N p :
     n < x -> prop n p ⊢ FUpd x A Es Es (inv n N p).
   Proof.
-    iIntros (LT) "P". iApply FUpd_alloc_gen. auto. iIntros. iFrame.
+    iIntros (LT) "P". iApply FUpd_alloc_gen; eauto.
   Qed.
 
   Lemma FUpd_open_aux x A Es n N E (LT : n < x) (INE : Es !! n = Some E) (IN : ↑N ⊆ E) p :
@@ -856,16 +1340,16 @@ Section FANCY_UPDATE.
     }
     iMod (wsats_OwnI_open x n i p LT with "[HI WSAT EN3]") as "(P & WSAT & DIS)".
     { iFrame. auto. }
-    iModIntro. iFrame. iPoseProof (OwnEs_union with "[ENS EN1]") as "ENS". iFrame.
+    iModIntro. iFrame. iPoseProof (OwnEs_union with "[ENS EN1]") as "ENS". { iFrame. }
     replace (∅ ∪ E ∖ ↑N) with (E ∖ ↑N). 2: set_solver.
     iFrame. iIntros "P (A & WSAT & EN1)".
     iMod (wsats_OwnI_close x n i p LT with "[HI WSAT P DIS]") as "(WSAT & EN3)".
     { iFrame. auto. }
     iModIntro. iFrame. iSplit; auto.
-    iPoseProof (OwnE_union with "[EN2 EN3]") as "EN2". iFrame.
+    iPoseProof (OwnE_union with "[EN2 EN3]") as "EN2". { iFrame. }
     rewrite <- union_difference_singleton_L; ss.
-    iPoseProof (OwnEs_union with "[EN1 EN2]") as "ENS". iFrame.
-    rewrite insert_id. iFrame. rewrite INE. f_equal.
+    iPoseProof (OwnEs_union with "[EN1 EN2]") as "ENS". { iFrame. }
+    rewrite insert_id. { iFrame. } rewrite INE. f_equal.
     rewrite difference_union_L. set_solver.
   Qed.
 
@@ -877,15 +1361,15 @@ Section FANCY_UPDATE.
   Proof.
     iIntros "[% (%iN & #HI)] (A & WSAT & ENS)".
     unfold lookup_def, subseteq_def in *. destruct (Es !! n) eqn:CASES; ss.
-    - iApply FUpd_open_aux; auto. unfold inv; auto. iFrame.
+    - iApply FUpd_open_aux; auto. { unfold inv; auto. } iFrame.
     - iAssert (
           (#=> (A ∗ (wsats x ∗ (OwnEs (<[n:=⊤ ∖ ↑N]> Es) ∗ (prop n p ∗ (prop n p -∗ FUpd x A (<[n:=⊤ ∖ ↑N]> Es) (<[n:=⊤]>Es) emp))))))
             -∗
             #=> (A ∗ (wsats x ∗ (OwnEs (<[n:=⊤ ∖ ↑N]> Es) ∗ (prop n p ∗ (prop n p -∗ FUpd x A (<[n:=⊤ ∖ ↑N]> Es) Es emp))))))%I as "K".
       { iIntros ">[A [SAT [ENS [P K]]]]". iModIntro. iFrame. iIntros "P".
         iPoseProof ("K" with "P") as "K". iIntros "[A [SAT ENS]]".
-        iPoseProof ("K" with "[A SAT ENS]") as ">[A [SAT [ENS _]]]". iFrame.
-        iMod (OwnEs_free with "ENS") as "ENS". auto.
+        iPoseProof ("K" with "[A SAT ENS]") as ">[A [SAT [ENS _]]]". { iFrame. }
+        iMod (OwnEs_free with "ENS") as "ENS"; eauto.
         iModIntro. iFrame.
       }
       iApply "K". iClear "K".
@@ -894,7 +1378,8 @@ Section FANCY_UPDATE.
       2:{ subst. rewrite insert_insert. auto. }
       iApply FUpd_open_aux; auto.
       { subst. apply lookup_insert. }
-      unfold inv; auto. iFrame.
+      { unfold inv; auto. }
+      { iFrame. }
   Qed.
 
   Lemma FUpd_intro x A Es P :
@@ -909,25 +1394,25 @@ Section FANCY_UPDATE.
          FUpd x A (<[n := (Es1 !? n) ∪ E]>Es1) (<[n := (Es2 !? n) ∪ E]>Es2) P.
   Proof.
     rewrite /FUpd. iIntros (D) "H (A & WSAT & ENS)".
-    iPoseProof ((OwnEs_acc_in _ n) with "ENS") as "[EN ENS]". apply lookup_insert.
+    iPoseProof ((OwnEs_acc_in _ n) with "ENS") as "[EN ENS]". { apply lookup_insert. }
     iPoseProof (OwnE_disjoint _ _ _ D with "EN") as "[EN1 EN]".
-    iPoseProof (OwnEs_union with "[ENS EN1]") as "ENS". iFrame.
+    iPoseProof (OwnEs_union with "[ENS EN1]") as "ENS". { iFrame. }
     replace (∅ ∪ lookup_def Es1 n) with (lookup_def Es1 n) by set_solver.
     destruct (coPset_equiv_dec E ∅); cycle 1.
     { unfold lookup_def, default in D. des_ifs; ss.
       2:{ exfalso. set_solver. }
       rewrite insert_insert. rewrite (insert_id Es1).
       2:{ unfold lookup_def, default. rewrite Heq. ss. }
-      iPoseProof ("H" with "[A WSAT ENS]") as ">(A & WSAT & ENS2 & P)". iFrame.
+      iPoseProof ("H" with "[A WSAT ENS]") as ">(A & WSAT & ENS2 & P)". { iFrame. }
       destruct (Es2 !! n) eqn:CASES.
       2:{ iMod ((OwnEs_acc_new _ _ CASES) with "ENS2") as "[EN2 _]".
-          iPoseProof (OwnE_exploit with "[EN EN2]") as "%DIS". iFrame.
+          iPoseProof (OwnE_exploit with "[EN EN2]") as "%DIS". { iFrame. }
           set_solver.
       }
       unfold lookup_def. rewrite CASES. ss.
       iPoseProof ((OwnEs_acc_in _ _ _ CASES) with "ENS2") as "[EN2 ENS]".
-      iPoseProof (OwnE_union with "[EN EN2]") as "EN". iFrame.
-      iPoseProof (OwnEs_union with "[ENS EN]") as "ENS". iFrame.
+      iPoseProof (OwnE_union with "[EN EN2]") as "EN". { iFrame. }
+      iPoseProof (OwnEs_union with "[ENS EN]") as "ENS". { iFrame. }
       replace (∅ ∪ (c0 ∪ E)) with (c0 ∪ E) by set_solver.
       iModIntro. iFrame.
     }
@@ -937,12 +1422,12 @@ Section FANCY_UPDATE.
       destruct (Es1 !! n) eqn:CASES.
       - rewrite (insert_id Es1).
         2:{ unfold lookup_def, default. rewrite CASES. ss. }
-        iPoseProof ("H" with "[A WSAT ENS]") as ">(A & WSAT & ENS2 & P)". iFrame.
+        iPoseProof ("H" with "[A WSAT ENS]") as ">(A & WSAT & ENS2 & P)". { iFrame. }
         iMod (OwnEs_lookup_def with "ENS2") as "ENS2". iModIntro. iFrame.
       - replace (lookup_def Es1 n) with (⊤ : coPset).
         2:{ unfold lookup_def, default. rewrite CASES. ss. }
         iMod ((OwnEs_free _ _ CASES) with "ENS") as "ENS".
-        iPoseProof ("H" with "[A WSAT ENS]") as ">(A & WSAT & ENS2 & P)". iFrame.
+        iPoseProof ("H" with "[A WSAT ENS]") as ">(A & WSAT & ENS2 & P)". { iFrame. }
         iMod (OwnEs_lookup_def with "ENS2") as "ENS2". iModIntro. iFrame.
     }
   Qed.
@@ -964,7 +1449,7 @@ Section FANCY_UPDATE.
          FUpd x A (<[n:=E1]>Es1) (<[n:=E2]>Es2) (FUpd x A (<[n:=E2]>Es3) (<[n:=E1]>Es3) P).
   Proof.
     rewrite /FUpd. iIntros (HE) "H (A & WSAT & ENS)".
-    iPoseProof ("H" with "[A WSAT ENS]") as ">(A & WSAT & ENS & P)". iFrame.
+    iPoseProof ("H" with "[A WSAT ENS]") as ">(A & WSAT & ENS & P)". { iFrame. }
     iModIntro.
     rewrite (union_difference_L _ _ HE).
     iPoseProof (OwnEs_disjoint with "ENS") as "[ENS EN]".
@@ -993,7 +1478,7 @@ Section FANCY_UPDATE.
   Proof.
     rewrite /FromModal /FUpd. ss.
     iIntros (HE) "P (A & WSAT & EN)".
-    iMod (OwnEs_alloc with "EN") as "EN". eauto. iModIntro. iFrame.
+    iMod (OwnEs_alloc with "EN") as "EN"; eauto. iModIntro. iFrame.
   Qed.
 
   Global Instance from_modal_FUpd_free x A Es n P :
@@ -1001,7 +1486,7 @@ Section FANCY_UPDATE.
   Proof.
     rewrite /FromModal /FUpd. ss.
     iIntros (HE) "P (A & WSAT & EN)".
-    iMod (OwnEs_free with "EN") as "EN". eauto. iModIntro. iFrame.
+    iMod (OwnEs_free with "EN") as "EN"; eauto. iModIntro. iFrame.
   Qed.
 
   Global Instance from_modal_FUpd_general x A Es n E1 E2 P :
@@ -1009,9 +1494,10 @@ Section FANCY_UPDATE.
   Proof.
     rewrite /FromModal /FUpd. ss.
     iIntros (HE) "P (A & WSAT & EN)". iModIntro. iFrame.
-    iPoseProof (OwnEs_acc_in with "EN") as "[EN ENS]". apply lookup_insert.
+    iPoseProof (OwnEs_acc_in with "EN") as "[EN ENS]". { apply lookup_insert. }
     iPoseProof ((OwnE_subset _ _ _ HE) with "EN") as "[EN1 _]".
-    iPoseProof (OwnEs_union with "[ENS EN1]") as "ENS". iFrame. rewrite insert_insert.
+    iPoseProof (OwnEs_union with "[ENS EN1]") as "ENS". { iFrame. }
+    rewrite insert_insert.
     replace (∅ ∪ E2) with E2 by set_solver. iFrame.
   Qed.
 
@@ -1037,7 +1523,7 @@ Use [FUpd_mask_frame] and [FUpd_intro_mask]")
     iIntros (LT) "[P K] I". inv LT.
     - rewrite /FUpd.
       iMod ("P" with "I") as "(A & WSAT & EN & P)". iApply ("K" with "P"). iFrame.
-    - iPoseProof (FUpd_mono n (S m) with "P") as "P". lia.
+    - iPoseProof (FUpd_mono n (S m) with "P") as "P". { lia. }
       rewrite /FUpd.
       iMod ("P" with "I") as "(A & WSAT & EN & P)". iApply ("K" with "P"). iFrame.
   Qed.
